WarblreEquiv/FunctTreeCompute/Equiv.v
@@ -2,11 +2,12 @@ From Linden Require Import EquivDef RegexpTranslation Regex LindenParameters
   Semantics FunctionalSemantics LWEquivTreeLemmas CharDescrCharSet Tactics
   NumericLemmas MSInput Chars Groups EquivLemmas Utils.
 From Warblre Require Import Parameters Semantics RegExpRecord Patterns
-  Node Result Notation Typeclasses List Base Node.
+  Node Result Notation Typeclasses List Base Node Match.
 Import Patterns.
 Import Result.Notations.
 Import Notation.
 Import NodeProps.Zipper.
+Import Match.
 From Coq Require Import ZArith PeanoNat Lia.
 
 Local Open Scope result_flow.
@@ -15,31 +16,32 @@ Section Equiv.
   Context `{characterClass: Character.class}.
 
   Lemma repeatMatcher'_done_equiv:
-    forall greedy parenIndex parenCount,
+    forall greedy parenIndex parenCount rer,
     forall (m: Matcher) (lreg: regex) (dir: Direction),
-      equiv_matcher m lreg dir ->
+      equiv_matcher m lreg rer dir ->
       def_groups lreg = List.seq (parenIndex + 1) parenCount ->
       forall fuel, equiv_matcher
         (fun ms mc => Semantics.repeatMatcher' m 0 (NoI.N 0) greedy ms mc parenIndex parenCount fuel)
-        (Regex.Quantified greedy 0 (NoI.N 0) lreg) dir.
+        (Regex.Quantified greedy 0 (NoI.N 0) lreg) rer dir.
   Proof.
-    intros greedy parenIndex parenCount m lreg dir Hequiv Hgroupsvalid fuel.
+    intros greedy parenIndex parenCount rer m lreg dir Hequiv Hgroupsvalid fuel.
     unfold equiv_matcher. intros str0 mc gl forbgroups act Hequivcont Hgldisj Hdef_forbid_disj.
-    unfold equiv_cont. intros gm ms inp res [|treefuel] t Hinpcompat Hgmms Hgmgl Hmsinp Hnoforbidden; simpl; try discriminate.
+    unfold equiv_cont. intros gm ms inp res [|treefuel] t Hinpcompat Hgmms Hgmgl Hmsinp Hmsvalid Hmsvalidchecks Hnoforbidden; simpl; try discriminate.
     destruct fuel as [|fuel]; simpl; try discriminate.
-    intros Hres Ht. eapply Hequivcont; eauto.
+    intros Hres Ht. eapply Hequivcont; eauto using ms_valid_wrt_checks_tail.
   Qed.
 
   Lemma repeatMatcher'_free_equiv:
-    forall greedy parenIndex parenCount,
+    forall greedy parenIndex parenCount rer,
     forall (m: Matcher) (lreg: regex) (dir: Direction),
-      equiv_matcher m lreg dir ->
+      equiv_matcher m lreg rer dir ->
+      MatcherInvariant.matcher_invariant m dir rer ->
       def_groups lreg = List.seq (parenIndex + 1) parenCount ->
       forall fuel delta, equiv_matcher
         (fun ms mc => Semantics.repeatMatcher' m 0 delta greedy ms mc parenIndex parenCount fuel)
-        (Regex.Quantified greedy 0 delta lreg) dir.
+        (Regex.Quantified greedy 0 delta lreg) rer dir.
     Proof.
-      intros greedy parenIndex parenCount m lreg dir Hequiv Hgroupsvalid fuel.
+      intros greedy parenIndex parenCount rer m lreg dir Hequiv MI Hgroupsvalid fuel.
       induction fuel as [|fuel IHfuel]. 1: discriminate.
 
       intro delta.
@@ -47,12 +49,12 @@ Section Equiv.
       1: { rewrite noi_eqb_eq in Hdeltazero. subst delta. now apply repeatMatcher'_done_equiv. }
       simpl. rewrite Hdeltazero.
       unfold equiv_matcher. intros str0 mc gl forbgroups act Hequivcont Hgldisj Hdef_forbid_disj.
-      unfold equiv_cont. intros gm ms inp res fueltree t Hinpcompat Hgmms Hgmgl Hmsinp Hnoforbidden.
+      unfold equiv_cont. intros gm ms inp res fueltree t Hinpcompat Hgmms Hgmgl Hmsinp Hvalidms Hmschecks Hnoforbidden.
       destruct List.Update.Nat.Batch.update as [cap'|] eqn:Heqcap'; simpl; try discriminate.
       set (mcloop := fun y: MatchState => if (_ =? _)%Z then _ else _).
       set (msreset := match_state _ _ cap').
-      assert (Hmcloopequiv: equiv_cont mcloop gl forbgroups (Acheck inp::Areg (Regex.Quantified greedy 0 (delta - 1)%NoI lreg)::act)%list dir str0). {
-        unfold equiv_cont. intros gm' ms' inp' res' fueltree' t' Hinp'compat Hgm'ms' Hgm'gl Hms'inp' Hnoforbidden'.
+      assert (Hmcloopequiv: equiv_cont mcloop gl forbgroups (Acheck inp::Areg (Regex.Quantified greedy 0 (delta - 1)%NoI lreg)::act)%list dir str0 rer). {
+        unfold equiv_cont. intros gm' ms' inp' res' fueltree' t' Hinp'compat Hgm'ms' Hgm'gl Hms'inp' Hms'valid Hms'checks Hnoforbidden'.
         unfold mcloop.
         destruct (_ =? _)%Z eqn:Heqcheck.
         - (* Case 1: the input has not progressed *)
@@ -69,13 +71,14 @@ Section Equiv.
           unfold equiv_cont in IHfuel.
           intros Hres'succ.
           destruct fueltree' as [|fueltree']; simpl; try discriminate.
-          (* Need matcher invariant *)
+          (* Follows from Hms'checks and other hypotheses linking ms', inp', inp and str0 *)
           replace (is_strict_suffix inp' inp dir) with true by admit.
           destruct compute_tree as [treecont|] eqn:Htreecontsucc; simpl; try discriminate.
           intro H. injection H as <-.
           simpl. eapply IHfuel; eauto.
-          replace (delta') with (delta-1)%NoI. 1: apply Htreecontsucc.
-          unfold delta'. now destruct delta.
+          all: replace (delta') with (delta-1)%NoI by now destruct delta.
+          + eauto using ms_valid_wrt_checks_tail.
+          + apply Htreecontsucc.
       }
       (* About m msreset mcloop *)
       unfold equiv_matcher in Hequiv. specialize (Hequiv str0 mcloop gl _ _ Hmcloopequiv Hgldisj).
@@ -103,7 +106,7 @@ Section Equiv.
             specialize_prove Hequiv. { eapply equiv_gm_ms_reset; eauto. reflexivity. }
             specialize_prove Hequiv. { eapply equiv_open_groups_reset; eauto. }
             specialize_prove Hequiv. { destruct ms. eapply ms_matches_inp_capchg; eauto. }
-            specialize_prove Hequiv by admit.
+            do 3 specialize_prove Hequiv by admit.
             specialize (Hequiv eq_refl Htitersucc).
             inversion Hequiv. simpl. unfold gmreset in H. rewrite <- H. simpl. constructor. assumption.
           * (* delta is infinite; copy-pasting and removing one line *)
@@ -114,7 +117,7 @@ Section Equiv.
             specialize_prove Hequiv. { eapply equiv_gm_ms_reset; eauto. reflexivity. }
             specialize_prove Hequiv. { eapply equiv_open_groups_reset; eauto. }
             specialize_prove Hequiv. { destruct ms. eapply ms_matches_inp_capchg; eauto. }
-            specialize_prove Hequiv by admit.
+            do 3 specialize_prove Hequiv by admit.
             specialize (Hequiv eq_refl Htitersucc).
             inversion Hequiv. simpl. unfold gmreset in H. rewrite <- H. simpl. constructor. assumption.
         + (* resloop is None *)
@@ -128,9 +131,9 @@ Section Equiv.
             specialize_prove Hequiv. { eapply equiv_gm_ms_reset; eauto. reflexivity. }
             specialize_prove Hequiv. { eapply equiv_open_groups_reset; eauto. }
             specialize_prove Hequiv. { destruct ms. eapply ms_matches_inp_capchg; eauto. }
-            specialize_prove Hequiv by admit.
+            do 3 specialize_prove Hequiv by admit.
             specialize (Hequiv eq_refl Htitersucc).
-            inversion Hequiv. simpl. unfold gmreset in H0. rewrite <- H0. simpl. eapply Hequivcont; eauto.
+            inversion Hequiv. simpl. unfold gmreset in H0. rewrite <- H0. simpl. eapply Hequivcont; eauto using ms_valid_wrt_checks_tail.
           * (* delta is infinite; copy-pasting and removing one line *)
             destruct (compute_tree _ inp (GroupMap.reset _ _) dir fueltree) as [titer|] eqn:Htitersucc; simpl; try discriminate.
             destruct (compute_tree act inp gm dir fueltree) as [tskip|] eqn:Htskipsucc; simpl; try discriminate.
@@ -139,9 +142,9 @@ Section Equiv.
             specialize_prove Hequiv. { eapply equiv_gm_ms_reset; eauto. reflexivity. }
             specialize_prove Hequiv. { eapply equiv_open_groups_reset; eauto. }
             specialize_prove Hequiv. { destruct ms. eapply ms_matches_inp_capchg; eauto. }
-            specialize_prove Hequiv by admit.
+            do 3 specialize_prove Hequiv by admit.
             specialize (Hequiv eq_refl Htitersucc).
-            inversion Hequiv. simpl. unfold gmreset in H0. rewrite <- H0. simpl. eapply Hequivcont; eauto.
+            inversion Hequiv. simpl. unfold gmreset in H0. rewrite <- H0. simpl. eapply Hequivcont; eauto using ms_valid_wrt_checks_tail.
       
       - destruct (mc ms) as [resskip|] eqn:Hresskipsucc; simpl; try discriminate.
         (* Probably similar to greedy case *)
@@ -149,15 +152,16 @@ Section Equiv.
   Admitted.
 
   Lemma repeatMatcher'_equiv:
-    forall greedy parenIndex parenCount,
+    forall greedy parenIndex parenCount rer,
     forall (m: Matcher) (lreg: regex) (dir: Direction),
-      equiv_matcher m lreg dir ->
+      equiv_matcher m lreg rer dir ->
+      MatcherInvariant.matcher_invariant m dir rer ->
       def_groups lreg = List.seq (parenIndex + 1) parenCount ->
       forall fuel min delta, equiv_matcher
         (fun ms mc => Semantics.repeatMatcher' m min (NoI.N min + delta)%NoI greedy ms mc parenIndex parenCount fuel)
-        (Regex.Quantified greedy min delta lreg) dir.
+        (Regex.Quantified greedy min delta lreg) rer dir.
   Proof.
-    intros greedy parenIndex parenCount m lreg dir Hequiv Hgroupsvalid fuel.
+    intros greedy parenIndex parenCount rer m lreg dir Hequiv MI Hgroupsvalid fuel.
     induction fuel as [|fuel IHfuel]. 1: discriminate.
 
     intros min delta.
@@ -176,12 +180,12 @@ Section Equiv.
     (* Now we have min <> 0 *)
     unfold equiv_matcher.
     intros str0 mc gl forbgroups act Hequivcont Hgldisj Hdef_forbid_disj. unfold equiv_cont.
-    intros gm ms inp res fueltree t Hinpcompat Hgmms Hgmgl Hmsinp Hnoforbidden.
+    intros gm ms inp res fueltree t Hinpcompat Hgmms Hgmgl Hmsinp Hmsvalid Hmschecks Hnoforbidden.
     simpl.
     rewrite Hmaxzero.
     replace (min' - 0) with min' by lia.
     destruct List.Update.Nat.Batch.update as [capreset|] eqn:Hcapreset; simpl; try discriminate.
-    rewrite mini_plus_plusminus_one with (mini := min') (plus := delta). 2: reflexivity.
+    rewrite mini_plus_plusminus_one with (mini := min') (plus := delta) by reflexivity.
     specialize (IHfuel min' delta). unfold equiv_matcher in IHfuel. specialize (IHfuel str0 mc gl forbgroups act Hequivcont Hgldisj Hdef_forbid_disj).
     unfold equiv_matcher in Hequiv. specialize (Hequiv str0 _ gl forbgroups _ IHfuel Hgldisj Hdef_forbid_disj).
     set (msreset := match_state _ _ capreset).
@@ -195,16 +199,19 @@ Section Equiv.
     - eapply equiv_open_groups_reset; eauto.
     - destruct ms. eapply ms_matches_inp_capchg; eauto.
     - admit.
+    - admit.
+    - admit.
   Admitted.
     
   Corollary repeatMatcher_equiv:
-    forall greedy parenIndex parenCount,
+    forall greedy parenIndex parenCount rer,
     forall (m: Matcher) (lreg: regex) (dir: Direction),
-      equiv_matcher m lreg dir ->
+      equiv_matcher m lreg rer dir ->
+      MatcherInvariant.matcher_invariant m dir rer ->
       def_groups lreg = List.seq (parenIndex + 1) parenCount ->
       forall min delta, equiv_matcher
         (fun ms mc => Semantics.repeatMatcher m min (NoI.N min + delta)%NoI greedy ms mc parenIndex parenCount)
-        (Regex.Quantified greedy min delta lreg) dir.
+        (Regex.Quantified greedy min delta lreg) rer dir.
   Proof.
   Admitted.
 
@@ -217,7 +224,10 @@ Section Equiv.
       (* and that dot matches all characters. *)
       (Hdotall: RegExpRecord.dotAll rer = true)
       (* Let lroot and wroot be a pair of equivanent regexes. *)
-      (root_equiv: equiv_regex wroot lroot),
+      (root_equiv: equiv_regex wroot lroot)
+      (* Assume that the conditions for the matcher invariant are met. *)
+      (Hcapcount: StaticSemantics.countLeftCapturingParensWithin wroot nil = RegExpRecord.capturingGroupsCount rer)
+      (HearlyErrors: EarlyErrors.Pass_Regex wroot nil),
       (* Then for any sub-regex wreg of the root Warblre regex, *)
     forall (wreg: Regex) (lreg: regex) ctx
       (Hroot: Root wroot (wreg, ctx))
@@ -227,9 +237,9 @@ Section Equiv.
         (* if compileSubPattern with direction dir yields a Matcher for regex wreg, *)
         (Hcompsucc: Semantics.compileSubPattern wreg ctx rer dir = Success m),
         (* then this Matcher is equivalent to the regex lreg and direction dir. *)
-        equiv_matcher m lreg dir.
+        equiv_matcher m lreg rer dir.
   Proof.
-    do 12 intro.
+    do 14 intro.
     remember (StaticSemantics.countLeftCapturingParensBefore _ _) as n in Hequiv.
     revert ctx Hroot Heqn.
     induction Hequiv as [
@@ -251,17 +261,17 @@ Section Equiv.
       intros ctx _ _ m dir. simpl.
       intro. injection Hcompsucc as <-.
       unfold equiv_matcher. intros str0 mc gl forbgroups act Hequivcont _ _.
-      unfold equiv_cont. intros gm ms inp res fuel t Hinpcompat Hgmms Hgmgl Hmsinp Hnoforbidden Hmcsucc.
+      unfold equiv_cont. intros gm ms inp res fuel t Hinpcompat Hgmms Hgmgl Hmsinp Hmsvalid Hmschecks Hnoforbidden Hmcsucc.
       destruct fuel as [|fuel]; try discriminate.
       simpl.
       intro Hsubtreesucc.
-      eauto using Hequivcont.
+      eapply Hequivcont; eauto using ms_valid_wrt_checks_tail.
   
     - (* Character; TODO generalize to all character descriptors *)
       intros ctx Hroot Heqn m dir Hcompsucc.
       injection Hcompsucc as <-.
       unfold equiv_matcher. intros str0 mc gl forbgroups act Hequivcont Hgldisj Hdef_forbid_disj.
-      unfold equiv_cont. intros gm ms inp res fuel t Hinpcompat Hgmms Hgmgl Hmsinp Hnoforbidden.
+      unfold equiv_cont. intros gm ms inp res fuel t Hinpcompat Hgmms Hgmgl Hmsinp Hmsvalid Hmschecks Hnoforbidden.
       unfold Semantics.characterSetMatcher.
       set (nextend := if (dir ==? forward)%wt then _ else _).
       destruct ((nextend <? 0)%Z || _)%bool eqn:Hoob; simpl.
@@ -282,6 +292,7 @@ Section Equiv.
           unfold equiv_cont in Hequivcont.
           rewrite advance_idx_advance_input with (inp' := inp') by assumption.
           eapply Hequivcont with (ms := match_state (MatchState.input ms) nextend (MatchState.captures ms)); eauto.
+          3,4: admit.
           1: eauto using advance_input_compat.
           eapply ms_matches_inp_adv; eauto. unfold MSInput.advance_ms. now destruct dir.
         * (* Read fails *)
@@ -321,7 +332,7 @@ Section Equiv.
       specialize (IH2 m2 dir Hcompsucc2).
       (* Introduce the required variables *)
       unfold equiv_matcher. intros str0 mc gl forbgroups act Hequivcont Hgldisj Hdef_forbid_disj.
-      unfold equiv_cont. intros gm ms inp res fuel t Hinpcompat Hgmms Hgmgl Hmsinp Hnoforbidden.
+      unfold equiv_cont. intros gm ms inp res fuel t Hinpcompat Hgmms Hgmgl Hmsinp Hmsvalid Hmschecks Hnoforbidden.
       unfold equiv_matcher in IH1, IH2.
       (* Specialize the induction hypotheses again naturally *)
       specialize (IH1 str0 mc gl forbgroups act Hequivcont).
@@ -336,8 +347,8 @@ Section Equiv.
       destruct m1 as [res1|] eqn:Hres1; simpl; try discriminate.
       destruct compute_tree as [t1|] eqn:Ht1; simpl; try discriminate.
       destruct (compute_tree (Areg lr2 :: act)%list _ _ _ _) as [t2|] eqn:Ht2; simpl; try discriminate.
-      specialize (IH1 gm ms inp res1 fuel t1 Hinpcompat Hgmms Hgmgl Hmsinp).
-      specialize_prove IH1 by admit. specialize (IH1 Hres1 Ht1).
+      specialize (IH1 gm ms inp res1 fuel t1 Hinpcompat Hgmms Hgmgl Hmsinp Hmsvalid).
+      do 2 specialize_prove IH1 by admit. specialize (IH1 Hres1 Ht1).
       (* Case analysis on whether the left branch matches *)
       destruct res1 as [msres1|] eqn:Hmsres1; simpl.
       + (* Left choice matches *)
@@ -348,7 +359,7 @@ Section Equiv.
         rename res into res2.
         intros Hres2 H. injection H as <-. simpl.
         inversion IH1 as [ HNone1 | ]. simpl.
-        eapply IH2; eauto. admit.
+        eapply IH2; eauto. all: admit.
 
     - (* Sequence *)
       intros ctx Hroot Heqn m dir. simpl.
@@ -368,11 +379,11 @@ Section Equiv.
       destruct dir; intro H; injection H as <-.
       + (* Forward *)
         unfold equiv_matcher. intros str0 mc gl forbgroups act Hequivcont Hgldisj Hdef_forbid_disj.
-        unfold equiv_cont. intros gm ms inp res [|fuel] t Hinpcompat Hgmms Hgmgl Hmsinp Hnoforbidden; try discriminate; simpl.
+        unfold equiv_cont. intros gm ms inp res [|fuel] t Hinpcompat Hgmms Hgmgl Hmsinp Hmsvalid Hmschecks Hnoforbidden; try discriminate; simpl.
         set (mc2 := fun s => _).
-        assert (Hequivcont2: equiv_cont mc2 gl (forbidden_groups lr2 ++ forbgroups) (Areg lr2 :: act)%list forward str0). {
-          unfold equiv_cont. clear gm ms inp res fuel t Hinpcompat Hgmms Hgmgl Hmsinp Hnoforbidden.
-          intros gm ms inp res fuel t Hinpcompat Hgmms Hgmgl Hmsinp Hnoforbidden. unfold mc2.
+        assert (Hequivcont2: equiv_cont mc2 gl (forbidden_groups lr2 ++ forbgroups) (Areg lr2 :: act)%list forward str0 rer). {
+          unfold equiv_cont. clear gm ms inp res fuel t Hinpcompat Hgmms Hgmgl Hmsinp Hmsvalid Hmschecks Hnoforbidden.
+          intros gm ms inp res fuel t Hinpcompat Hgmms Hgmgl Hmsinp Hmsvalid Hmschecks Hnoforbidden. unfold mc2.
           intros Hres Ht. eapply IH2; eauto.
           1: eauto using disj_parent_disj_child, Child_Sequence_right.
           admit.
@@ -383,11 +394,11 @@ Section Equiv.
 
       + (* Backward *)
         unfold equiv_matcher. intros str0 mc gl forbgroups act Hequivcont Hgldisj Hdef_forbid_disj.
-        unfold equiv_cont. intros gm ms inp res [|fuel] t Hinpcompat Hgmms Hgmgl Hmsinp Hnoforbidden; try discriminate; simpl.
+        unfold equiv_cont. intros gm ms inp res [|fuel] t Hinpcompat Hgmms Hgmgl Hmsinp Hmsvalid Hmschecks Hnoforbidden; try discriminate; simpl.
         set (mc1 := fun s => _).
-        assert (Hequivcont1: equiv_cont mc1 gl (forbidden_groups lr1 ++ forbgroups) (Areg lr1 :: act)%list backward str0). {
-          unfold equiv_cont. clear gm ms inp res fuel t Hinpcompat Hgmms Hgmgl Hmsinp Hnoforbidden.
-          intros gm ms inp res fuel t Hinpcompat Hgmms Hgmgl Hmsinp Hnoforbidden. unfold mc1.
+        assert (Hequivcont1: equiv_cont mc1 gl (forbidden_groups lr1 ++ forbgroups) (Areg lr1 :: act)%list backward str0 rer). {
+          unfold equiv_cont. clear gm ms inp res fuel t Hinpcompat Hgmms Hgmgl Hmsinp Hmsvalid Hmschecks Hnoforbidden.
+          intros gm ms inp res fuel t Hinpcompat Hgmms Hgmgl Hmsinp Hmsvalid Hmschecks Hnoforbidden. unfold mc1.
           intros Hres Ht. eapply IH1; eauto.
           1: eauto using disj_parent_disj_child, Child_Sequence_left.
           admit.
@@ -417,6 +428,10 @@ Section Equiv.
       rewrite Heqn in Hgroupsvalid. replace (StaticSemantics.countLeftCapturingParensBefore _ _) with parenIndex in Hgroupsvalid. 2: {
         unfold parenIndex, StaticSemantics.countLeftCapturingParensBefore. reflexivity.
       }
+      assert (MIsub: MatcherInvariant.matcher_invariant msub dir rer). {
+        eapply MatcherInvariant.compileSubPattern with (root := wroot) (r := wr); eauto.
+        eauto using Down.same_root_down0, Down_Quantified_inner.
+      }
       inversion Hequivquant as [
           Heqwquant Heqlquant |
           Heqwquant Heqlquant |
@@ -432,10 +447,10 @@ Section Equiv.
       destruct Semantics.compileSubPattern as [msub | ] eqn:Hcompsuccsub; simpl; try discriminate.
       intro H. injection H as <-.
       unfold equiv_matcher. intros str0 mc gl forbgroups act Hequivcont Hgldisj Hdef_forbid_disj.
-      unfold equiv_cont. intros gm ms inp res [|fuel] t Hinpcompat Hgmms Hgmgl Hmsinp Hnoforbidden; simpl; try discriminate.
+      unfold equiv_cont. intros gm ms inp res [|fuel] t Hinpcompat Hgmms Hgmgl Hmsinp Hmsvalid Hmschecks Hnoforbidden; simpl; try discriminate.
       set (mcclose := fun (y: MatchState) => _).
-      assert (Hequivmcclose: equiv_cont mcclose ((S n, idx inp)::gl)%list forbgroups (Aclose (S n)::act)%list dir str0). {
-        unfold equiv_cont. intros gm' ms' inp' res' [|fuel'] t' Hinp'compat Hgm'ms' Hgm'gl' Hms'inp' Hnoforbidden'; simpl; try discriminate.
+      assert (Hequivmcclose: equiv_cont mcclose ((S n, idx inp)::gl)%list forbgroups (Aclose (S n)::act)%list dir str0 rer). {
+        unfold equiv_cont. intros gm' ms' inp' res' [|fuel'] t' Hinp'compat Hgm'ms' Hgm'gl' Hms'inp' Hms'valid Hms'checks Hnoforbidden'; simpl; try discriminate.
         destruct compute_tree as [treecont|] eqn:Htreecont; simpl; try discriminate.
         unfold mcclose.
         set (rres := if (dir ==? forward)%wt then _ else _). destruct rres as [r|] eqn:Hrres; simpl; try discriminate.
@@ -448,6 +463,8 @@ Section Equiv.
         - eapply equiv_open_groups_close_group; eauto.
         - eapply ms_matches_inp_close_group; eauto.
         - admit.
+        - admit.
+        - admit.
       }
       destruct compute_tree as [treecont|] eqn:Htreecont; simpl; try discriminate.
       intros Hres H. injection H as <-. simpl.
@@ -458,6 +475,7 @@ Section Equiv.
       + admit.
       + admit. (* Group map equivalence after opening a group *)
       + admit. (* Group map equivalence to open groups after opening a group *)
+      + admit.
       + admit.
 
     - (* Lookaround *)
